src/tls/cmitls.c
@@ -23,22 +23,26 @@ const char *option_hostname;
 int option_port;
 
 #define OPTION_LIST \
-	STRING_OPTION("-v", version, "sets maximum protocol version to <1.0 | 1.1 | 1.2 | 1.3> (default: 1.3)") \
-	STRING_OPTION("-mv", minversion, "sets minimum protocol version to <1.0 | 1.1 | 1.2 | 1.3> (default: 1.2)") \
-	BOOL_OPTION("-s", isserver, "run as server instead of client") \
-	BOOL_OPTION("-no_early_data", 0rtt, "disable early data (server support and client offer)") \
-	STRING_OPTION("-psk", psk, "L:K add an entry in the PSK database at label L with key K (in hex), associtated with the fist current -cipher") \
-	STRING_OPTION("-offerpsk", offerpsk, "offer the given PSK identifier(s) (must be loaded first with --psk). Client only.") \
-	BOOL_OPTION("-verify", verify, "enforce peer certificate validation") \
-	BOOL_OPTION("-noems", noems, "disable extended master secret in TLS <= 1.2 (client only)") \
+    STRING_OPTION("-v", version, "sets maximum protocol version to <1.0 | 1.1 | 1.2 | 1.3> (default: 1.3)") \
+    STRING_OPTION("-mv", minversion, "sets minimum protocol version to <1.0 | 1.1 | 1.2 | 1.3> (default: 1.2)") \
+    BOOL_OPTION("-s", isserver, "run as server instead of client") \
+    BOOL_OPTION("-0rtt", 0rtt, "enable early data (server support and client offer)") \
+    STRING_OPTION("-psk", psk, "L:K add an entry in the PSK database at label L with key K (in hex), associtated with the fist current -cipher") \
+    STRING_OPTION("-ticket", ticket, "T:K add ticket T in the PSK database with RMS K (in hex), associated with the first current -cipher") \
+    STRING_OPTION("-offerpsk", offerpsk, "offer the given PSK identifier(s) (must be loaded first with --psk). Client only.") \
+    BOOL_OPTION("-verify", verify, "enforce peer certificate validation") \
+    BOOL_OPTION("-noems", noems, "disable extended master secret in TLS <= 1.2 (client only)") \
     STRING_OPTION("-ciphers", ciphers, "colon-separated list of cipher suites; see above for valid values") \
     STRING_OPTION("-sigalgs", sigalgs, "colon-separated list of signature algorithms; see above for valid values") \
+    STRING_OPTION("-alpn", alpn, "colon-separated list of application-level protocols") \
+    BOOL_OPTION("-quic", quic, "test QUIC API, using the QuicTransportParameters extension") \
+    BOOL_OPTION("-reconnect", reconnect, "reconnect at the end of the session, using received ticket (client only)") \
     STRING_OPTION("-groups", groups, "colon-separated list of named groups; see above for valid values") \
     STRING_OPTION("-cert", cert, "PEM file containing certificate chain to send") \
     STRING_OPTION("-key", key, "PEM file containing private key of endpoint certificate in chain") \
     STRING_OPTION("-CAFile", cafile, "set openssl root cert file to <path>")
 
-// Declare global variables representing the options	
+// Declare global variables representing the options
 #define STRING_OPTION(n, var, help) const char *option_##var;
 #define BOOL_OPTION(n, var, help)   int option_##var;
 OPTION_LIST
@@ -49,13 +53,13 @@ OPTION_LIST
 #define STRING_OPTION(n, var, help) { n, &option_##var, NULL, help },
 #define BOOL_OPTION(n, var, help)   { n, NULL, &option_##var, help },
 struct {
-	const char *OptionName;		// name of the option switch
-	const char **String;		// place to store the option argument string, or NULL if no argument follows
-	int *Boolean;				// if String==NULL, then this is the place to store a boolean '1'
-	const char *HelpText;		// help text for the option
+    const char *OptionName;     // name of the option switch
+    const char **String;        // place to store the option argument string, or NULL if no argument follows
+    int *Boolean;               // if String==NULL, then this is the place to store a boolean '1'
+    const char *HelpText;       // help text for the option
 } Options[] = {
-	OPTION_LIST
-	{}
+    OPTION_LIST
+    {}
 };
 #undef STRING_OPTION
 #undef BOOL_OPTION
@@ -68,12 +72,12 @@ typedef struct {
 // Print the usage text
 void PrintUsage(void)
 {
-	size_t i=0;
+    size_t i=0;
 
-    printf("Usage:  cmitls.exe [options] hostname port\n");	
-	for (i=0; Options[i].OptionName; ++i) {
-		printf("  %-10s %s\n", Options[i].OptionName, Options[i].HelpText);
-	}
+    printf("Usage:  cmitls.exe [options] hostname port\n");
+    for (i=0; Options[i].OptionName; ++i) {
+        printf("  %-10s %s\n", Options[i].OptionName, Options[i].HelpText);
+    }
 }
 
 const char *hostname_arg;
@@ -84,406 +88,674 @@ const char *port_arg;
 //  ArgsRemaining - the number of elements in argvRemaining
 //  argvRemaining - the remaining arguments
 //
-// Returns -1 for failure, or 1 or 2, to report the number 
+// Returns -1 for failure, or 1 or 2, to report the number
 // of arguments consumed
 int ParseArg(const char *Name, int ArgsRemaining, char **argvRemaining)
 {
-	size_t i=0;
-	
-	for (i=0; Options[i].OptionName; ++i) {
-		if (strcmp(Options[i].OptionName, Name) == 0) {
-			if (Options[i].String) {
-				if (ArgsRemaining) {
-					*(Options[i].String) = argvRemaining[0];
-				} else {
-					return -1;
-				}
-				return 2;
-			} else {
-				*(Options[i].Boolean) = 1;
-				return 1;
-			}
-		}
-	}
-	printf("Unknown option: %s\n", Name);
-	return -1; // Unknown option
+    size_t i=0;
+
+    for (i=0; Options[i].OptionName; ++i) {
+        if (strcmp(Options[i].OptionName, Name) == 0) {
+            if (Options[i].String) {
+                if (ArgsRemaining) {
+                    *(Options[i].String) = argvRemaining[0];
+                } else {
+                    return -1;
+                }
+                return 2;
+            } else {
+                *(Options[i].Boolean) = 1;
+                return 1;
+            }
+        }
+    }
+    printf("Unknown option: %s\n", Name);
+    return -1; // Unknown option
 }
 
 // Parse the command line arguments
 // Returns -1 for failure, 0 for success
 int ParseArgs(int argc, char **argv)
 {
-	int i = 1;
-	int result;
-	
-	while (i < argc) {
-		if (argv[i][0] == '-') {
-			result = ParseArg(argv[i], argc-i-1, &argv[i+1]);
-			if (result == -1) {
-				return -1;
-			}
-			i += result;
-		} else if (hostname_arg == NULL) {
-			hostname_arg = argv[i++];
-		} else if (port_arg == NULL) {
-			port_arg = argv[i++];
-		} else {
-			printf("Unknown argument: %s\n", argv[i]);
-			return -1;
-		}
-	}
-	
-	if (hostname_arg) {
-		option_hostname = hostname_arg;
-	} else {
-		option_hostname = (option_isserver) ? "0.0.0.0" : "127.0.0.1";
-	}
-	if (port_arg) {
-		option_port = atoi(port_arg);
-	} else {
-		option_port = 443;
-	}
-	return 0;
+    int i = 1;
+    int result;
+
+    while (i < argc) {
+        if (argv[i][0] == '-') {
+            result = ParseArg(argv[i], argc-i-1, &argv[i+1]);
+            if (result == -1) {
+                return -1;
+            }
+            i += result;
+        } else if (hostname_arg == NULL) {
+            hostname_arg = argv[i++];
+        } else if (port_arg == NULL) {
+            port_arg = argv[i++];
+        } else {
+            printf("Unknown argument: %s\n", argv[i]);
+            return -1;
+        }
+    }
+
+    if (hostname_arg) {
+        option_hostname = hostname_arg;
+    } else {
+        option_hostname = (option_isserver) ? "0.0.0.0" : "127.0.0.1";
+    }
+    if (port_arg) {
+        option_port = atoi(port_arg);
+    } else {
+        option_port = 443;
+    }
+    return 0;
 }
 
 void PrintErrors(char *out_msg, char *err_msg)
 {
-	if (out_msg) {
-		printf("MITLS: %s", out_msg);
-		FFI_mitls_free_msg(out_msg);
-	}
-	if (err_msg) {
-		fprintf(stderr, "MITLS: %s", err_msg);
-		FFI_mitls_free_msg(err_msg);
-	}
+    if (out_msg) {
+        printf("MITLS: %s", out_msg);
+        FFI_mitls_free_msg(out_msg);
+    }
+    if (err_msg) {
+        fprintf(stderr, "MITLS: %s", err_msg);
+        FFI_mitls_free_msg(err_msg);
+    }
 }
 
 int Configure(mitls_state **pstate)
 {
-	char *out_msg;
-	char *err_msg;
-	mitls_state *state;
-	int r;
-	
-	*pstate = NULL;
-	
-	r = FFI_mitls_configure(&state, option_version, option_hostname, &out_msg, &err_msg);
-	PrintErrors(out_msg, err_msg);
-	if (r == 0) {
-		printf("FFI_mitls_configure(%s,%s) failed.\n", option_version, option_hostname);
-		return 2;
-	}
-	if (option_cert) {
-		r = FFI_mitls_configure_cert_chain_file(state, option_cert);
-		if (r == 0) {
-			printf("FFI_mitls_configure_cert_chain_file(%s) failed.\n", option_cert);
-			return 2;
-		}
-	}
-	if (option_key) {
-		r = FFI_mitls_configure_private_key_file(state, option_key);
-		if (r == 0) {
-			printf("FFI_mitls_configure_private_key_file(%s) failed.\n", option_key);
-			return 2;
-		}
-	}
-	if (option_cafile) {
-		r = FFI_mitls_configure_ca_file(state, option_cafile);
-		if (r == 0) {
-			printf("FFI_mitls_configure_ca_file(%s) failed.\n", option_cafile);
-			return 2;
-		}
-	}
-	if (option_ciphers) {
-		r = FFI_mitls_configure_cipher_suites(state, option_ciphers);
-		if (r == 0) {
-			printf("FFI_mitls_configure_cipher_suites(%s) failed.\n", option_ciphers);
-			return 2;
-		}
-	}
-	if (option_sigalgs) {
-		r = FFI_mitls_configure_signature_algorithms(state, option_sigalgs);
-		if (r == 0) {
-			printf("FFI_mitls_configure_signature_algorithms(%s) failed.\n", option_sigalgs);
-			return 2;
-		}
-	}
-	if (option_groups) {
-		r = FFI_mitls_configure_named_groups(state, option_groups);
-		if (r == 0) {
-			printf("FFI_mitls_configure_named_groups(%s) failed.\n", option_groups);
-			return 2;
-		}
-	}
-	*pstate = state;
-	return 0;
+    char *out_msg;
+    char *err_msg;
+    mitls_state *state;
+    int r;
+
+    *pstate = NULL;
+
+    if (option_quic) {
+        r = FFI_mitls_quic_configure(&state,
+        65536, // max_stream_data
+        16777216, // max_data
+        256, // max_stream_id
+        60, // idle_timeout
+        0, // max_packet_size (use default value)
+        option_hostname,
+        &out_msg, &err_msg);
+    } else {
+        r = FFI_mitls_configure(&state, option_version, option_hostname, &out_msg, &err_msg);
+    }
+    PrintErrors(out_msg, err_msg);
+    if (r == 0) {
+        printf("FFI_mitls_configure(%s,%s) failed.\n", option_version, option_hostname);
+        return 2;
+    }
+    if (option_cert) {
+        r = FFI_mitls_configure_cert_chain_file(state, option_cert);
+        if (r == 0) {
+            printf("FFI_mitls_configure_cert_chain_file(%s) failed.\n", option_cert);
+            return 2;
+        }
+    }
+    if (option_key) {
+        r = FFI_mitls_configure_private_key_file(state, option_key);
+        if (r == 0) {
+            printf("FFI_mitls_configure_private_key_file(%s) failed.\n", option_key);
+            return 2;
+        }
+    }
+    if (option_cafile) {
+        r = FFI_mitls_configure_ca_file(state, option_cafile);
+        if (r == 0) {
+            printf("FFI_mitls_configure_ca_file(%s) failed.\n", option_cafile);
+            return 2;
+        }
+    }
+    if (option_ciphers) {
+        r = FFI_mitls_configure_cipher_suites(state, option_ciphers);
+        if (r == 0) {
+            printf("FFI_mitls_configure_cipher_suites(%s) failed.\n", option_ciphers);
+            return 2;
+        }
+    }
+    if (option_sigalgs) {
+        r = FFI_mitls_configure_signature_algorithms(state, option_sigalgs);
+        if (r == 0) {
+            printf("FFI_mitls_configure_signature_algorithms(%s) failed.\n", option_sigalgs);
+            return 2;
+        }
+    }
+    if (option_groups) {
+        r = FFI_mitls_configure_named_groups(state, option_groups);
+        if (r == 0) {
+            printf("FFI_mitls_configure_named_groups(%s) failed.\n", option_groups);
+            return 2;
+        }
+    }
+
+    if (option_0rtt) {
+        r = FFI_mitls_configure_early_data(state, 1);
+        if (r == 0) {
+            printf("FFI_mitls_configure_early_data(true) failed.\n");
+            return 2;
+        }
+    }
+
+    if (option_psk) {
+        printf("-psk is not yet implemented in cmitls\n");
+        return 2;
+    }
+
+    if (option_ticket) {
+        printf("-ticket is not yet implemented in cmitls\n");
+        return 2;
+    }
+
+    if (option_offerpsk) {
+        printf("-offerpsk is not yet implemented in cmitls\n");
+        return 2;
+    }
+
+    if (option_alpn) {
+        r = FFI_mitls_configure_alpn(state, option_alpn);
+        if (r == 0) {
+            printf("FFI_mitls_configure_alpn(%s) failed.\n", option_alpn);
+            return 2;
+        }
+    }
+
+    *pstate = state;
+    return 0;
 }
 
 // Callback from miTLS, when it is ready to send a message via the socket
 int SendCallback(struct _FFI_mitls_callbacks *callbacks, const void *buffer, size_t buffer_size)
 {
-	callback_context *ctx = (callback_context*)callbacks;
-	ssize_t r;
-	
-	r = send(ctx->sockfd, buffer, buffer_size, 0);
-	if (r != buffer_size) {
-		printf("Error %d returned from socket send()\n", WSAGetLastError());
-	}
-	return (int)r;
+    callback_context *ctx = (callback_context*)callbacks;
+    ssize_t r;
+
+    r = send(ctx->sockfd, buffer, buffer_size, 0);
+    if (r != buffer_size) {
+        printf("Error %d returned from socket send()\n", WSAGetLastError());
+    }
+    return (int)r;
 }
 
 // Callback from miTLS, when it is ready to receive a message via the socket
 int RecvCallback(struct _FFI_mitls_callbacks *callbacks, void *buffer, size_t buffer_size)
 {
-	callback_context *ctx = (callback_context*)callbacks;
-	ssize_t r;
-	
-	r = recv(ctx->sockfd, buffer, buffer_size, 0);
-	if (r != buffer_size) {
-		printf("Error %d returned from socket recv()\n", WSAGetLastError());
-	}
-	return (int)r;
+    callback_context *ctx = (callback_context*)callbacks;
+    ssize_t r;
+
+    r = recv(ctx->sockfd, buffer, buffer_size, 0);
+    if (r != buffer_size) {
+        printf("Error %d returned from socket recv()\n", WSAGetLastError());
+    }
+    return (int)r;
 }
 
 #define MAX_RECEIVED_REQUEST_LENGTH  (65536) // 64kb
 int SingleServer(mitls_state *state, SOCKET clientfd)
 {
-	callback_context ctx;
-	char *out_msg;
-	char *err_msg;
-	void *db;
-	size_t db_length;
-	int r;
-	size_t payload_length;
-	char *payload;
-	
-	const char ctext[] = "You are connected to miTLS*!\r\n"
-                         "This is the request you sent:\r\n\r\n";	
-    const char cpayload[] = "HTTP/1.1 200 OK\r\nConnection: close\r\nContent-Length:%d\r\n"
-	                        "Content-Type: text/plain; charset=utf-8\r\n\r\n";
-		
-	ctx.cb.send = SendCallback;
-	ctx.cb.recv = RecvCallback;
-	ctx.sockfd = clientfd;
-	r = FFI_mitls_accept_connected(&ctx.cb, state, &out_msg, &err_msg);
-	PrintErrors(out_msg, err_msg);
-	if (r == 0) {
-		printf("FFI_mitls_accept_connected() failed\n");
-		return 1;
-	}
-	db = FFI_mitls_receive(state, &db_length, &out_msg, &err_msg);
-	if (db == NULL) {
-		printf("FFI_mitls_receive() failed\n");
-		return 1;
-	}
-	printf("Received data:\n");
-	puts((const char *)db);
-	
-	// Truncate overly long client requests
-	if (db_length > MAX_RECEIVED_REQUEST_LENGTH) {
-		db_length = MAX_RECEIVED_REQUEST_LENGTH;
-	}
-	
-	// Determine the payload length.  This length is the maximum... the actual
-	// length may be a few bytes less due to differing db_length-to-string conversions.
-	// +5 for the number of characters needed to render text for the max db_length of 65536.
-	payload_length=sizeof(ctext) + sizeof(cpayload) + db_length + 5;
-	payload = (char*)_alloca(payload_length);
-	sprintf(payload, cpayload, (int)(sizeof(ctext)+db_length-1) /* not counting the '\0' at the end of ctext */);
-	strcat(payload, ctext);
-	strncat(payload, (const char*)db, db_length);
+    callback_context ctx;
+    char *out_msg;
+    char *err_msg;
+    void *db;
+    size_t db_length;
+    int r;
+    size_t payload_length;
+    char *payload;
 
-	FFI_mitls_free_msg(db);
-	
-	r = FFI_mitls_send(state, payload, strlen(payload), &out_msg, &err_msg);
-	PrintErrors(out_msg, err_msg);
-	if (r == 0) {
-		printf("FFI_mitls_send() failed\n");
-		return 1;
-	}
-	FFI_mitls_close(state);
-	return 0;
+    const char ctext[] = "You are connected to miTLS*!\r\n"
+                         "This is the request you sent:\r\n\r\n";
+    const char cpayload[] = "HTTP/1.1 200 OK\r\nConnection: close\r\nContent-Length:%d\r\n"
+                            "Content-Type: text/plain; charset=utf-8\r\n\r\n";
+
+    ctx.cb.send = SendCallback;
+    ctx.cb.recv = RecvCallback;
+    ctx.sockfd = clientfd;
+    r = FFI_mitls_accept_connected(&ctx.cb, state, &out_msg, &err_msg);
+    PrintErrors(out_msg, err_msg);
+    if (r == 0) {
+        printf("FFI_mitls_accept_connected() failed\n");
+        return 1;
+    }
+    db = FFI_mitls_receive(state, &db_length, &out_msg, &err_msg);
+    if (db == NULL) {
+        printf("FFI_mitls_receive() failed\n");
+        return 1;
+    }
+    printf("Received data:\n");
+    puts((const char *)db);
+
+    // Truncate overly long client requests
+    if (db_length > MAX_RECEIVED_REQUEST_LENGTH) {
+        db_length = MAX_RECEIVED_REQUEST_LENGTH;
+    }
+
+    // Determine the payload length.  This length is the maximum... the actual
+    // length may be a few bytes less due to differing db_length-to-string conversions.
+    // +5 for the number of characters needed to render text for the max db_length of 65536.
+    payload_length=sizeof(ctext) + sizeof(cpayload) + db_length + 5;
+    payload = (char*)_alloca(payload_length);
+    sprintf(payload, cpayload, (int)(sizeof(ctext)+db_length-1) /* not counting the '\0' at the end of ctext */);
+    strcat(payload, ctext);
+    strncat(payload, (const char*)db, db_length);
+
+    FFI_mitls_free_msg(db);
+
+    r = FFI_mitls_send(state, payload, strlen(payload), &out_msg, &err_msg);
+    PrintErrors(out_msg, err_msg);
+    if (r == 0) {
+        printf("FFI_mitls_send() failed\n");
+        return 1;
+    }
+    FFI_mitls_close(state);
+    return 0;
 }
 
 int TestServer()
 {
-	SOCKET sockfd;
-	struct hostent *host;
-	struct sockaddr_in addr;
-	mitls_state *state;
-	
-	printf("===============================================\n Starting test TLS server...\n");
-	
-	host = gethostbyname(option_hostname);
-	if (host == NULL) {
-		printf("Failed gethostbyname(%s) %d\n", option_hostname, WSAGetLastError());
-		return 1;
-	}
-	memset(&addr, 0, sizeof(addr));
-	addr.sin_family = AF_INET;
-	memcpy(&addr.sin_addr.s_addr, host->h_addr, host->h_length);
-	addr.sin_port = htons(option_port);	
-	
-	sockfd = socket(AF_INET, SOCK_STREAM, 0);
-	if (sockfd < 0) {
-		printf("Failed socket open: %d\n", WSAGetLastError());
-		return 1;
-	}
-	if (bind(sockfd, (struct sockaddr *)&addr, sizeof(addr)) < 0) {
-		printf("Failed bind() %d\n", WSAGetLastError());
-		closesocket(sockfd);
-		return 1;
-	}
-	if (listen(sockfd, 128) < 0) {
-		printf("Failed listen() %d\n", WSAGetLastError());
-		closesocket(sockfd);
-		return 1;
-	}
-	while (1) {
-		SOCKET clientsockfd;
-		socklen_t len = sizeof(addr);
-		
-		clientsockfd = accept(sockfd, (struct sockaddr*)&addr, &len);
-		if (clientsockfd == SOCKET_ERROR) {
-			printf("Failed accept() %d\n", WSAGetLastError());
-			closesocket(sockfd);
-			return 1;
-		}
-		if (Configure(&state) != 0) {
-			return 1;
-		}
-		if (SingleServer(state, clientsockfd)) {
-			return 1;
-		}
-		closesocket(clientsockfd);
-	}
-	return 0;
+    SOCKET sockfd;
+    struct hostent *host;
+    struct sockaddr_in addr;
+    mitls_state *state;
+
+    printf("===============================================\n Starting test TLS server...\n");
+
+    host = gethostbyname(option_hostname);
+    if (host == NULL) {
+        printf("Failed gethostbyname(%s) %d\n", option_hostname, WSAGetLastError());
+        return 1;
+    }
+    memset(&addr, 0, sizeof(addr));
+    addr.sin_family = AF_INET;
+    memcpy(&addr.sin_addr.s_addr, host->h_addr, host->h_length);
+    addr.sin_port = htons(option_port);
+
+    sockfd = socket(AF_INET, SOCK_STREAM, 0);
+    if (sockfd < 0) {
+        printf("Failed socket open: %d\n", WSAGetLastError());
+        return 1;
+    }
+    if (bind(sockfd, (struct sockaddr *)&addr, sizeof(addr)) < 0) {
+        printf("Failed bind() %d\n", WSAGetLastError());
+        closesocket(sockfd);
+        return 1;
+    }
+    if (listen(sockfd, 128) < 0) {
+        printf("Failed listen() %d\n", WSAGetLastError());
+        closesocket(sockfd);
+        return 1;
+    }
+    while (1) {
+        SOCKET clientsockfd;
+        socklen_t len = sizeof(addr);
+
+        clientsockfd = accept(sockfd, (struct sockaddr*)&addr, &len);
+        if (clientsockfd == SOCKET_ERROR) {
+            printf("Failed accept() %d\n", WSAGetLastError());
+            closesocket(sockfd);
+            return 1;
+        }
+        if (Configure(&state) != 0) {
+            return 1;
+        }
+        if (SingleServer(state, clientsockfd)) {
+            return 1;
+        }
+        closesocket(clientsockfd);
+    }
+    return 0;
+}
+
+// auxiliary reading loop (brittle when using TCP)
+void quic_recv_until(mitls_state *state, int p)
+{
+    int r;
+
+    do {
+        char *out_msg;
+        char *err_msg;
+        r = FFI_mitls_quic_process(state, &out_msg, &err_msg);
+        PrintErrors(out_msg, err_msg);
+        switch (r) {
+        case TLS_would_block: printf("would block\n"); break;
+        case TLS_error_local: printf("fatal error\n"); break; // bugbug: print 'e'
+        case TLS_error_alert: printf("received fatal alert\n"); break; // bugbug: print 'e'
+        case TLS_client_early: printf("client offers early data\n"); break; // bugbug: print 'secret0'
+        case TLS_client_complete: printf("client completes X: the server Y early data\n"); break; // bugbug: secret1, b
+        case TLS_server_accept: printf("server accepts X early data\n"); break; // bugbug: secret0/secret1 and true/false
+        case TLS_server_complete: printf("server completes\n"); break;
+        default: printf("Unknown return %d from FFI_mitls_quic_process\n", r); return;
+        }
+    } while (r != p);
+}
+
+void print_bytes(const void *buf, size_t len)
+{
+    const unsigned char *b = (const unsigned char*)buf;
+
+    for (size_t i=0; i<len; ++i) {
+        printf("%2.2x ", b[i]);
+    }
+}
+
+void quic_dump(mitls_state *state)
+{
+    printf("OK\n");
+    void* secret0;
+    void* secret1;
+    size_t secret0_size;
+    size_t secret1_size;
+    char *out_msg;
+    char *err_msg;
+
+    secret0 = FFI_mitls_quic_get_exporter(state, 0, &secret0_size, &out_msg, &err_msg);
+    PrintErrors(out_msg, err_msg);
+    secret1 = FFI_mitls_quic_get_exporter(state, 1, &secret1_size, &out_msg, &err_msg);
+    PrintErrors(out_msg, err_msg);
+
+    if (secret0) {
+        printf("early secret: ");
+        print_bytes(secret0, secret0_size);
+        printf("\n");
+    }
+    if (secret1) {
+        printf("main secret: ");
+        print_bytes(secret1, secret1_size);
+        printf("\n");
+    }
+    FFI_mitls_free_packet(secret0);
+    FFI_mitls_free_packet(secret1);
+
+    // bugbug: dump get_parameters of state for Client and Server  via FFI_mitls_quic_get_parameters()
+}
+
+int TestQuicClient(void)
+{
+    mitls_state *state;
+    SOCKET sockfd;
+    struct hostent *peer;
+    struct sockaddr_in addr;
+    callback_context ctx;
+    char *out_msg;
+    char *err_msg;
+    int r;
+
+    printf("CLIENT\n");
+
+    sockfd = socket(AF_INET, SOCK_STREAM, 0);
+    if (sockfd < 0) {
+        printf("Failed socket open: %s\n", strerror(errno));
+        return 1;
+    }
+    peer = gethostbyname(option_hostname);
+    if (peer == NULL) {
+        printf("Failed gethostbyname %s\n", strerror(errno));
+        return 1;
+    }
+    memset(&addr, 0, sizeof(addr));
+    addr.sin_family = AF_INET;
+    memcpy(&addr.sin_addr.s_addr, peer->h_addr, peer->h_length);
+    addr.sin_port = htons(option_port);
+
+    if (connect(sockfd, (struct sockaddr*)&addr, sizeof(addr)) < 0) {
+        printf("Failed connect %s\n", strerror(errno));
+        return 1;
+    }
+
+    r = Configure(&state);
+    if (r != 0) {
+        return 1;
+    }
+
+    ctx.cb.send = SendCallback;
+    ctx.cb.recv = RecvCallback;
+    ctx.sockfd = sockfd;
+    r = FFI_mitls_quic_create_client(&ctx.cb, state, &out_msg, &err_msg);
+    PrintErrors(out_msg, err_msg);
+    if (r == 0) {
+        printf("FFI_mitls_quic_create_client() failed\n");
+        return 1;
+    }
+
+    quic_recv_until(state, TLS_client_complete);
+    quic_recv_until(state, TLS_would_block); // ticket_sending
+    quic_recv_until(state, TLS_would_block);
+    quic_recv_until(state, TLS_would_block);
+    quic_dump(state);
+
+    return 0;
+}
+
+#define MAX_RECEIVED_REQUEST_LENGTH  (65536) // 64kb
+int SingleQuicServer(mitls_state *state, SOCKET clientfd)
+{
+    callback_context ctx;
+    char *out_msg;
+    char *err_msg;
+    void *db;
+    size_t db_length;
+    int r;
+
+    ctx.cb.send = SendCallback;
+    ctx.cb.recv = RecvCallback;
+    ctx.sockfd = clientfd;
+    r = FFI_mitls_quic_create_server(&ctx.cb, state, &out_msg, &err_msg);
+    PrintErrors(out_msg, err_msg);
+    if (r == 0) {
+        printf("FFI_mitls_quic_create_server() failed\n");
+        return 1;
+    }
+
+    // brittle, as we need to write the ticket without blocking on TCP read.
+    quic_recv_until(state, TLS_server_complete);
+    quic_recv_until(state, TLS_would_block);
+    quic_dump(state);
+
+    FFI_mitls_close(state);
+    return 0;
+}
+
+int TestQuicServer(void)
+{
+    SOCKET sockfd;
+    struct hostent *host;
+    struct sockaddr_in addr;
+    mitls_state *state;
+
+    printf("SERVER\n");
+
+    host = gethostbyname(option_hostname);
+    if (host == NULL) {
+        printf("Failed gethostbyname(%s) %d\n", option_hostname, WSAGetLastError());
+        return 1;
+    }
+    memset(&addr, 0, sizeof(addr));
+    addr.sin_family = AF_INET;
+    memcpy(&addr.sin_addr.s_addr, host->h_addr, host->h_length);
+    addr.sin_port = htons(option_port);
+
+    sockfd = socket(AF_INET, SOCK_STREAM, 0);
+    if (sockfd < 0) {
+        printf("Failed socket open: %d\n", WSAGetLastError());
+        return 1;
+    }
+    if (bind(sockfd, (struct sockaddr *)&addr, sizeof(addr)) < 0) {
+        printf("Failed bind() %d\n", WSAGetLastError());
+        closesocket(sockfd);
+        return 1;
+    }
+    if (listen(sockfd, 128) < 0) {
+        printf("Failed listen() %d\n", WSAGetLastError());
+        closesocket(sockfd);
+        return 1;
+    }
+    while (1) {
+        SOCKET clientsockfd;
+        socklen_t len = sizeof(addr);
+
+        clientsockfd = accept(sockfd, (struct sockaddr*)&addr, &len);
+        if (clientsockfd == SOCKET_ERROR) {
+            printf("Failed accept() %d\n", WSAGetLastError());
+            closesocket(sockfd);
+            return 1;
+        }
+        if (Configure(&state) != 0) {
+            return 1;
+        }
+        if (SingleQuicServer(state, clientsockfd)) {
+            return 1;
+        }
+        closesocket(clientsockfd);
+    }
+    return 0;
 }
 
 int TestClient(void)
 {
-	mitls_state *state;
-	SOCKET sockfd;
-	struct hostent *peer;
-	struct sockaddr_in addr;
-	int requestlength;
-	ssize_t r;
-	callback_context ctx;
-	char *out_msg;
-	char *err_msg;
-	char request[512];
-	void *response;
-	size_t response_length;
+    mitls_state *state;
+    SOCKET sockfd;
+    struct hostent *peer;
+    struct sockaddr_in addr;
+    int requestlength;
+    ssize_t r;
+    callback_context ctx;
+    char *out_msg;
+    char *err_msg;
+    char request[512];
+    void *response;
+    size_t response_length;
 
-	printf("===============================================\n");
-	printf("Starting test client...\n");
-	
-	const char request_template[] = "GET / HTTP/1.1\r\nHost: %s\r\n\r\n";
-	if (sizeof(request_template) + strlen(option_hostname) >= sizeof(request)) {
-		// Host name is too long
-		printf("Host name is too long.\n");
-		return 1;
-	}
-	requestlength = sprintf(request, request_template, option_hostname);
-	
-	sockfd = socket(AF_INET, SOCK_STREAM, 0);
-	if (sockfd < 0) {
-		printf("Failed socket open: %s\n", strerror(errno));
-		return 1;
-	}
-	peer = gethostbyname(option_hostname);
-	if (peer == NULL) {
-		printf("Failed gethostbyname %s\n", strerror(errno));
-		return 1;
-	}
-	memset(&addr, 0, sizeof(addr));
-	addr.sin_family = AF_INET;
-	memcpy(&addr.sin_addr.s_addr, peer->h_addr, peer->h_length);
-	addr.sin_port = htons(option_port);
-	
-	if (connect(sockfd, (struct sockaddr*)&addr, sizeof(addr)) < 0) {
-		printf("Failed connect %s\n", strerror(errno));
-		return 1;
-	}
+    printf("===============================================\n");
+    printf("Starting test client...\n");
 
-	r = Configure(&state);
-	if (r != 0) {
-		return 1;
-	}
-	
-	ctx.cb.send = SendCallback;
-	ctx.cb.recv = RecvCallback;
-	ctx.sockfd = sockfd;
-	r = FFI_mitls_connect(&ctx.cb, state, &out_msg, &err_msg);
-	PrintErrors(out_msg, err_msg);
-	if (r == 0) {
-		printf("FFI_mitls_connect() failed\n");
-		return 1;
-	}
-	
-	printf("Read OK, sending HTTP request...\n");
-	r = FFI_mitls_send(state, request, requestlength, &out_msg, &err_msg);
-	PrintErrors(out_msg, err_msg);
-	if (r == 0) {
-		printf("FFI_mitls_send() failed\n");
-		closesocket(sockfd);
-		return 1;
-	}
-	
-	response = FFI_mitls_receive(state, &response_length, &out_msg, &err_msg);
-	if (response == NULL) {
-		printf("FFI_mitls_receive() failed\n");
-		closesocket(sockfd);
-		return 1;
-	}
-	printf("Received data:\n");
-	puts((const char *)response);
-	FFI_mitls_free_msg(response);
-	
-	printf("Closing connection, irrespective of the response\n");
-	FFI_mitls_close(state);
-	closesocket(sockfd);
-	
-	return 0;
+    const char request_template[] = "GET / HTTP/1.1\r\nHost: %s\r\n\r\n";
+    if (sizeof(request_template) + strlen(option_hostname) >= sizeof(request)) {
+        // Host name is too long
+        printf("Host name is too long.\n");
+        return 1;
+    }
+    requestlength = sprintf(request, request_template, option_hostname);
+
+    sockfd = socket(AF_INET, SOCK_STREAM, 0);
+    if (sockfd < 0) {
+        printf("Failed socket open: %s\n", strerror(errno));
+        return 1;
+    }
+    peer = gethostbyname(option_hostname);
+    if (peer == NULL) {
+        printf("Failed gethostbyname %s\n", strerror(errno));
+        return 1;
+    }
+    memset(&addr, 0, sizeof(addr));
+    addr.sin_family = AF_INET;
+    memcpy(&addr.sin_addr.s_addr, peer->h_addr, peer->h_length);
+    addr.sin_port = htons(option_port);
+
+    if (connect(sockfd, (struct sockaddr*)&addr, sizeof(addr)) < 0) {
+        printf("Failed connect %s\n", strerror(errno));
+        return 1;
+    }
+
+    r = Configure(&state);
+    if (r != 0) {
+        return 1;
+    }
+
+    ctx.cb.send = SendCallback;
+    ctx.cb.recv = RecvCallback;
+    ctx.sockfd = sockfd;
+    r = FFI_mitls_connect(&ctx.cb, state, &out_msg, &err_msg);
+    PrintErrors(out_msg, err_msg);
+    if (r == 0) {
+        printf("FFI_mitls_connect() failed\n");
+        return 1;
+    }
+
+    printf("Read OK, sending HTTP request...\n");
+    r = FFI_mitls_send(state, request, requestlength, &out_msg, &err_msg);
+    PrintErrors(out_msg, err_msg);
+    if (r == 0) {
+        printf("FFI_mitls_send() failed\n");
+        closesocket(sockfd);
+        return 1;
+    }
+
+    response = FFI_mitls_receive(state, &response_length, &out_msg, &err_msg);
+    if (response == NULL) {
+        printf("FFI_mitls_receive() failed\n");
+        closesocket(sockfd);
+        return 1;
+    }
+    printf("Received data:\n");
+    puts((const char *)response);
+    FFI_mitls_free_msg(response);
+
+    printf("Closing connection, irrespective of the response\n");
+    FFI_mitls_close(state);
+    closesocket(sockfd);
+
+    return 0;
 }
 
 int main(int argc, char **argv)
 {
-	int r;
-	
+    int r;
+
 #if _WIN32
 {
-	WSADATA wsaData;
-	r = WSAStartup(MAKEWORD(2,2), &wsaData);
-	if (r != 0) {
-		printf("WSAStartup failed: %d\n", r);
-		return 2;
-	}
+    WSADATA wsaData;
+    r = WSAStartup(MAKEWORD(2,2), &wsaData);
+    if (r != 0) {
+        printf("WSAStartup failed: %d\n", r);
+        return 2;
+    }
 }
-#endif	
-	
-	option_version = "1.3";
-	if (ParseArgs(argc, argv) != 0) {
-		PrintUsage();
-		return 1;
-	}
+#endif
 
-	if (option_minversion) {
-		printf("Warning: -mv is not supported via FFI yet.  Ignored.\n");
-	}
-	
-	r = FFI_mitls_init();
-	if (r == 0) {
-		printf("FFI_mitls_init() failed!\n");
-		return 2;
-	}
-	
-	if (option_isserver) {
-		r = TestServer();
-	} else {
-		r = TestClient();
-	}
-	FFI_mitls_cleanup();
+    option_version = "1.3";
+    if (ParseArgs(argc, argv) != 0) {
+        PrintUsage();
+        return 1;
+    }
 
-	return r;
+    if (option_minversion) {
+        if (strcmp(option_minversion, option_version)) {
+            printf("Warning: -mv is not supported via FFI yet.  Ignored.\n");
+        }
+    }
+
+    r = FFI_mitls_init();
+    if (r == 0) {
+        printf("FFI_mitls_init() failed!\n");
+        return 2;
+    }
+
+    if (option_isserver) {
+        if (option_quic) {
+            r = TestQuicServer();
+        } else {
+            r = TestServer();
+        }
+    } else {
+        if (option_quic) {
+            r = TestQuicClient();
+        } else {
+            r = TestClient();
+        }
+        if (option_reconnect) {
+            // This needs access to Ticket.lookup
+            printf("-reconnect is not supported in cmitls\n");
+            r = 3;
+        } else {
+            if (option_quic) {
+                r = TestQuicClient();
+            } else {
+                r = TestClient();
+            }
+        }
+    }
+    FFI_mitls_cleanup();
+
+    return r;
 }
