src/tls/test/mitls.ml
@@ -155,7 +155,7 @@ let _ =
     ("-s", Arg.Unit (fun () -> role := Server), "run as server instead of client");
     ("-0rtt", Arg.Unit (fun () -> config := {!config with enable_early_data = true;}), "enable early data (server support and client offer)");
     ("-psk", Arg.String (fun s -> load_psk false s), " L:K add an entry in the PSK database at label L with key K (in hex), associated with the fist current -cipher");
-    ("-ticket", Arg.String (fun s -> load_psk true s), " T:K add ticket T in the PSK database with RMS K (in hex), associated with the fist current -cipher");
+    ("-ticket", Arg.String (fun s -> load_psk true s), " T:K add ticket T in the PSK database with RMS K (in hex), associated with the first current -cipher");
     ("-offerpsk", Arg.String (fun s -> offer_psk s), "offer the given PSK identifier(s) (must be loaded first with -psk or -ticket, 1.3 client only)");
     ("-tlsapi", Arg.Unit (fun () -> ()), "run through the TLS API (legacy, always on)");
     ("-verify", Arg.Unit (fun () -> config := {!config with check_peer_certificate = true;}), "enforce peer certificate validation");
